\section*{Auxiliary Lemmata}
\begin{lemma}[Sequential Command Soundness]\label{lem:seqSoundness}
For all $\seq{1} \in \Seqs$, $\left(\Hp{1}, \seq{1}, \Hp{2}\right) \in \AxiomsSeq$ and $\h{} \in \Heaps$:
%
\[
	\opSemSeq{\seq{1}}{\reifyH{\Hp{1} \composeH \{\h{}\}}} \subseteq \reifyH{\Hp{2} \composeH \{\h{}\}}
\]
%
\begin{proof}
By induction over the structure of $\seq{}$. Pick an arbitrary $\h{} \in \Heaps$.\\

\noindent\textbf{Case \hspace*{0.3cm}}\bc{}\\
This follows from parameter \ref{par:basicSoundness}.\\


\noindent\textbf{Case \hspace*{0.3cm}\skipC}\\
\textbf{RTS.}
%
\[
	\opSemSeq{\seq{1}}{\reifyH{\Hp{} \composeH \{\h{}\}}} 
	\subseteq \reifyH{\Hp{} \composeH \{\h{}\}}
\]
%
\begin{proof}
%
\[
\begin{array}{r l}
	\opSemSeq{\seq{1}}{\reifyH{\Hp{} \composeH \{\h{}\}}} 
	= &
	\reifyH{\Hp{} \composeH \{\h{}\}}\\

	\subseteq & \reifyH{\Hp{} \composeH \{\h{}\}}
\end{array}
\]
%
as required.
\renewcommand{\qed}{}
\end{proof}
%
%

\noindent\textbf{Case \hspace*{0.3cm}}$\seq{1} ; \seq{2}$\\
\textbf{RTS.}
%
\[
	\opSemSeq{\seq{1}; \seq{2}}{\reifyH{\Hp{} \composeH \{\h{}\}}} 
	\subseteq \reifyH{\Hp{}' \composeH \{\h{}\}}
\]
%
where $\left(\Hp{}, \seq{1}, \Hp{}'' \right), \left(\Hp{}'', \seq{2}, \Hp{}' \right)  \in \AxiomsSeq$.
\begin{proof}
%
\[
\begin{array}{r l}
	
	\opSemSeq{\seq{1}; \seq{2}}{\reifyH{\Hp{} \composeH \{\h{}\}}} 
	= &  
	\opSemSeq{\seq{2}}{ \opSemSeq{\seq{1}}{\reifyH{\Hp{} \composeH \{\h{}\}}}}\\

	\text{(I.H.) \hspace*{0.5cm}}
	\subseteq &
	\opSemSeq{\seq{2}}{\reifyH{\Hp{}'' \composeH \{\h{}\}}}\\
	
	\text{(I.H.) \hspace*{0.5cm}}
	\subseteq &
	\reifyH{\Hp{}' \composeH \{\h{}\}}
	
\end{array}
\]
%
as required.
\renewcommand{\qed}{}
\end{proof}
%
%

\noindent\textbf{Case \hspace*{0.3cm}}$\seq{1} + \seq{2}$\\
\textbf{RTS.}
%
\[
	\opSemSeq{\seq{1} + \seq{2}}{\reifyH{\Hp{} \composeH \{\h{}\}}} 
	\subseteq \reifyH{\Hp{}' \composeH \{\h{}\}}
\]
%
where $\left(\Hp{}, \seq{1}, \Hp{}' \right), \left(\Hp{}, \seq{2}, \Hp{}' \right)  \in \AxiomsSeq$.
\begin{proof}
%
\[
\hspace*{-0.2cm}
\begin{array}{r l}
	
	\opSemSeq{\seq{1} + \seq{2}}{\reifyH{\Hp{} \composeH \{\h{}\}}} 
	= &  
	\opSemSeq{\seq{1}}{\reifyH{\Hp{} \composeH \{\h{}\}}} \;\cup\; \opSemSeq{\seq{2}}{\reifyH{\Hp{} \composeH \{\h{}\}}}\\

	\text{(I.H.) \hspace*{0.5cm}}
	\subseteq &
	\reifyH{\Hp{}' \composeH \{\h{}\}} \;\cup\; \reifyH{\Hp{}' \composeH \{\h{}\}}\\
	
	\subseteq &
	\reifyH{\Hp{}' \composeH \{\h{}\}}
	
\end{array}
\]
%
as required.
\renewcommand{\qed}{}
\end{proof}
%
%

\noindent\textbf{Case \hspace*{0.3cm}}$\seq{}^{*}$\\
\textbf{RTS.}
%
\[
	\opSemSeq{\seq{}^{*}}{\reifyH{\Hp{} \composeH \{\h{}\}}} 
	\subseteq \reifyH{\Hp{} \composeH \{\h{}\}}
\]
%
where $\left(\Hp{}, \seq{}, \Hp{} \right)  \in \AxiomsSeq$.
\begin{proof}
%
\[
\begin{array}{r l}
	
	\opSemSeq{\seq{}^{*}}{\reifyH{\Hp{} \composeH \{\h{}\}}} 
	= &  
	\opSemSeq{\skipC + \seq{}; \seq{}^{*}}{\reifyH{\Hp{} \composeH \{\h{}\}}} \\
	
	= & \opSemSeq{\skipC}{\reifyH{\Hp{} \composeH \{\h{}\}}} 
		\cup \opSemSeq{\seq{}; \seq{}^{*}}{\reifyH{\Hp{} \composeH \{\h{}\}}} \\

	\text{(I.H.) \hspace*{0.5cm}}
	\subseteq &
	\reifyH{\Hp{} \composeH \{\h{}\}} \cup \reifyH{\Hp{} \composeH \{\h{}\}}\\
	
	\subseteq &
	\reifyH{\Hp{} \composeH \{\h{}\}}
	
\end{array}
\]
%
as required.
\renewcommand{\qed}{}
\end{proof}
%
%
\end{proof}
\end{lemma}
%
%
\input{Soundness/Atomic/guaranteeContainment.tex}
%
%
\begin{lemma}\label{lemma:contextSwitch}
%
\[
\begin{array}{l}
	\for{p, q, r \in \LStates} \for{\amod{}, \amod{}' \in \AMods} \for{n \in \Nats}\\
	\hspace*{0.5cm} \extendsAMUpto{\amod{}, \amod{L}}{n}{p \composeL q}{r}{\amod{}'} \implies 
									\extendsAMUpto{\amod{}, \amod{L}}{n}{p}{q \composeL r}{\amod{}'}
\end{array}
\]
%
\begin{proof} By induction on number of steps $n$.

\noindent Pick an arbitrary $p, q, r \in \LStates, \amod{}, \amod{}' \in \AMods$.\\

\noindent\textbf{Base case}\\
\textbf{RTS. }\hspace*{0.5cm}$\extendsAMUpto{\amod{}, \amod{L}}{0}{p \composeL q}{r}{\amod{}'} \implies \extendsAMUpto{\amod{}, \amod{L}}{0}{p}{q \composeL r}{\amod{}'}$\\
This holds trivially by definition of $\extendsAMUpto{\amod{}, \amod{L}}{0}{p}{q \composeL r}{\amod{}'}$\\

\noindent\textbf{Inductive Step} Pick an arbitrary $n \in \Nats$, then
%
\begin{equation}
	\tag{I.H.}
	\extendsAMUpto{\amod{}, \amod{L}}{(n-1)}{p \composeL q}{r}{\amod{}'} \implies 
	\extendsAMUpto{\amod{}, \amod{L}}{(n-1)}{p}{q \composeL r}{\amod{}'}
\label{L1:IH}
\end{equation}
%
Assume:
%
\begin{align}
	& \extendsAMUpto{\amod{}, \amod{L}}{n}{p \composeL q}{r}{\amod{}'} \label{L1:Ass1}
\end{align}
%
Show
%
\begin{align}
	&\for{\ca{}, c, d, t, l_3, l_4} \for{(l_1 \composeL f, l_2 \composeL f) \in \amod{}'(\ca{})} \nonumber\\
	&\hspace*{0.2cm}\left(\for{l'} l' \leq l_1 \land l' \leq l_2 \implies l' = \unitL\right)\;\land\; l_1 \composeL f \leq  p \composeL q \composeL r \composeL t \;\land\\
	&\hspace*{0.2cm}  l_1 = l_3 \composeL l_4 \;\land\; l_1 \maxMeetL p \composeL q = l_3 \;\land\; p \composeL q = l_3 \composeL c \;\land\; r = l_4 \composeL d \implies \nonumber\\
	&\hspace*{0.5cm} \extendsAMUpto{\amod{}, \amod{L}}{(n-1)}{l_2 \composeL c}{d}{\amod{}'}\\
	&\hspace*{0.5cm}\land\;t = \unitL \implies (l_1 \composeL c \composeL d, l_2 \composeL c \composeL d) \in \amod{}(\ca{}) \lor l_2 \composeL c \composeL d \text{ is undefined} \label{L1:Goal1}\\ \nonumber\\
	& \begin{array}{l}
		\for{\ca{}} \for{(l_1 \composeL f, l_2 \composeL f) \in \amod{L}(\ca{})} \for{c, d} \\
  \hspace*{0.2cm} l_1 \composeL f \composeL c = p \composeL q \composeL r \composeL d \;\land\; \left(\for{l'} l' \leq l_0 \land l' \leq l'_0 \implies l' = \unitL\right)  \;\implies\\
  \hspace*{0.4cm}\exsts{f', c'} (l_1 \composeL f', l_2 \composeL f') \in \amod{}'(\ca{}) \;\land\; l_1 \composeL f' \composeL c' =  p \composeL q \composeL r \composeL d\\
		\hspace*{0.4cm}\lor\;l_2 \composeL f \composeL c \text{ is undefined}\\
		\hspace*{0.4cm}\lor\; \exsts{r'} l_2 \composeL f \composeL c = p \composeL r' \composeL d \;\land\; \extendsAMUpto{\amod{G}, \amod{L}}{(m-1)}{p}{r'}{\amod{}'}
	\end{array}
	\label{L1:Goal2}\\\nonumber
\end{align}
%
\textbf{RTS. (\ref{L1:Goal1})}\\
Pick an arbitrary $\ca{}, c, d, t, l_3, l_4, (l_1 \composeL f, l_2 \composeL f) \in \amod{}'(\ca{})$ such that
%
\begin{align}
	&\for{l'} l' \leq l_1 \land l' \leq l_2 \implies l' = \unitL \label{L1:Ass10}\\
	& l_1 = l_3 \composeL l_4 \label{L1:Ass11}\\
	& p = l_3 \composeL c \label{L1:Ass12}\\
	& q \composeL r = l_4 \composeL d \label{L1:Ass13}
\end{align}
%(\ref{L1:Ass})
Since $l_4 \leq q \composeL r$ (\ref{L1:Ass13}), from Lemma \ref{lem:divideUpper} we have:
%
\begin{align}
	\exsts{l_5, l_6, e, g} \hspace*{0.5cm} & l_4 = l_5 \composeL l_6 \label{L1:Ass15}\\
	& q = l_5 \composeL e \label{L1:Ass16}\\
	& r = l_6 \composeL g \label{L1:Ass17}
\end{align}
%
From (\ref{L1:Ass13}), (\ref{L1:Ass15})-(\ref{L1:Ass17}) and cancellativity of separation algebra of \LStates\ we have:
%
\begin{align}
	e \composeL g = d \label{L1:Ass18}
\end{align}
%
From (\ref{L1:Ass1}), (\ref{L1:Ass10})-(\ref{L1:Ass17}) and assumption of case 1 we have:
%
\begin{align}
	&\extendsAMUpto{\amod{}, \amod{L}}{(n-1)}{l_2 \composeL c \composeL e}{g}{\amod{}'} \;\land \nonumber\\
	& t = \unitL \implies (l_1 \composeL c \composeL  d, l_2 \composeL c \composeL d) \in \amod{}(\ca{}) \lor\; (l_2 \composeL c \composeL d) \hspace*{0.2cm}\text{is undefined} \nonumber
\end{align}
%(\ref{L1:Ass})
From (\ref{L1:IH}) and (\ref{L1:Ass18}) we can rewrite the above as 
%
\begin{align}
	&\extendsAMUpto{\amod{}, \amod{L}}{(n-1)}{l_2 \composeL c}{d}{\amod{}'} \;\land \nonumber\\
	& t = \unitL \implies (l_1 \composeL c \composeL  d, l_2 \composeL c \composeL d) \in \amod{}(\ca{}) \lor\; (l_2 \composeL c \composeL d) \hspace*{0.2cm}\text{is undefined} \nonumber
\end{align}\\
%(\ref{L1:Ass})
%
%
%
%

\noindent\textbf{RTS. (\ref{L1:Goal2})}\\
Pick an arbitrary $\ca{}, l_1, l_2, f, c, d$ such that:
%
\begin{align}
	\begin{array}{l}
		l_1 \composeL f \composeL c = p \composeL q \composeL r \composeL d\\
		\left(\for{l'} l' \leq l_1 \land l' \leq l_2 \implies l' = \unitL\right)\\
  	(l_1 \composeL f, l_2 \composeL f) \in \amod{L}(\ca{}) \\
	\end{array} \label{LCS: Ass1}
\end{align} 
%
From (\ref{L1:Ass1}) we have:
%
\[
\begin{array}{l}
	\exsts{f', c'} (l_1 \composeL f', l_2 \composeL f') \in \amod{}'(\ca{}) \;\land\; l_1 \composeL f' \composeL c' =  p \composeL q \composeL r \composeL d\\
	\lor\;l_2 \composeL f \composeL c \text{ is undefined}\\
	\lor\; \exsts{r'} l_2 \composeL f \composeL c = p \composeL q \composeL r' \composeL d \;\land\;\extendsAMUpto{\amod{G}, \amod{L}}{(m-1)}{p \composeL q}{r'}{\amod{}'}
\end{array}
\]
%
From (\ref{L1:IH}) we can rewrite the above as: 
%
\[
\begin{array}{l}
	\exsts{f', c'} (l_1 \composeL f', l_2 \composeL f') \in \amod{}'(\ca{}) \;\land\; l_1 \composeL f' \composeL c' =  p \composeL q \composeL r \composeL d\\
	\lor\;l_2 \composeL f \composeL c \text{ is undefined}\\
	\lor\; \exsts{r'} l_2 \composeL f \composeL c = p \composeL q \composeL r' \composeL d \;\land\; \extendsAMUpto{\amod{G}, \amod{L}}{(m-1)}{p}{q \composeL r'}{\amod{}'}
\end{array}
\]
%
and consequently,
%
\[
\begin{array}{l}
	\exsts{f', c'} (l_1 \composeL f', l_2 \composeL f') \in \amod{}'(\ca{}) \;\land\; l_1 \composeL f' \composeL c' =  p \composeL q \composeL r \composeL d\\
	\lor\;l_2 \composeL f \composeL c \text{ is undefined}\\
	\lor\; \exsts{r'} l_2 \composeL f \composeL c = p \composeL r' \composeL d \;\land\; \extendsAMUpto{\amod{G}, \amod{L}}{(m-1)}{p}{r'}{\amod{}'}
\end{array}
\]
%
as required.
\end{proof}
\end{lemma}
%
%
\begin{lemma}[] \label{lem:amodHiding} \todo Update
%
\[
\begin{array}{l}
	\for{l, r \in \LStates} \for{\amod{0}, \amod{1}, \amod{} \in \AMods} \for{ F \in \pset{\LStates}} \for{n \in \Nats} \\
	
	\hspace*{0.5cm} 
	l \in F \;\land\; 
	F \fences \amod{0} \;\land\; 
	\amod{0} \weakenI{F} \amod{1}\;\land\;
	\extendsAMUpto{\amod{}, \amod{L}}{n}{l}{r}{\amod{0}}\\
	
	\hspace*{1.5cm} \implies\\
	
	
	\hspace*{0.5cm}
	\extendsAMUpto{\amod{}, \amod{L} \cup \amod{1}}{n}{l}{r}{\amod{1}}\\
\end{array}
\]
%
\begin{proof}
By induction on $n$. \\
Pick an arbitrary $l, r \in \LStates,\ \amod{0}, \amod{1}, \amod{} \in \AMods,\  F \in \pset{\LStates}$;\\
\noindent\textbf{Base case} $n = 0$\\
\textbf{RTS. } $\extendsAMUpto{\amod{}, \amod{L} \cup \amod{1}}{0}{l}{r}{\amod{1}}$\\
This case holds trivially from the definition of $\extendsAMUpto{\amod{}, \amod{L} \cup \amod{1}}{0}{l}{r}{\amod{1}}$.\\

\noindent\textbf{Inductive Case}\\
\textbf{Assume}
\begin{align}
	&l \in F \label{L2:Ass1}\\
	&F \fences \amod{0} \label{L2:Ass2}\\
%	&F \fences \amod{1} \label{L2:Ass3}\\
	&\amod{0} \weakenI{F} \amod{1}\label{L2:Ass4}\\
	& \extendsAMUpto{\amod{}, \amod{L}}{n}{l}{r}{\amod{0}} \label{L2:Ass5}\\
%
	&\for{l, r \in \LStates} l \in F \land F \fences \amod{0} \land \amod{0} \weakenI{F} \amod{1} \land \extendsAMUpto{\amod{}, \amod{L}}{(n-1)}{l}{r}{\amod{0}}
	\implies \nonumber\\
	&\hspace*{1cm}\extendsAMUpto{\amod{}, \amod{L} \cup \amod{1}}{(n-1)}{l}{r}{\amod{1}} \tag{I.H}\label{L2:I.H}\\\nonumber
\end{align}

\noindent\textbf{Show}
\begin{align}
	&\for{\ca{}, c, d, t, l_3, l_4}\for{(l_1 \composeL f, l_2 \composeL f) \in \amod{1}(\ca{})} \nonumber\\
	&\hspace*{0.2cm} \left(\for{l'} l' \leq l_1 \land l' \leq l_2 \implies l' = \unitL\right)\;\land\; l_1 \composeL f \leq  l \composeL r \composeL t \;\land \nonumber\\
	&\hspace*{0.2cm}  l_1 = l_3 \composeL l_4 \;\land\; l_1 \maxMeetL l = l_3 \;\land\; l = l_3 \composeL c \;\land\; r = l_4 \composeL d\implies \nonumber\\
	& \hspace*{0.4cm} \extendsAMUpto{\amod{}, \amod{L} \cup \amod{1}}{(n-1)}{l_2 \composeL c}{d}{\amod{1}} \nonumber\\
	& \hspace*{0.4cm}\land\; t = \unitL \implies (l_1 \composeL c \composeL d, l_2 \composeL c \composeL d) \in \amod{}(\ca{}) \lor l_2 \composeL c \composeL d \text{ is undefined} 
\label{L2:Goal1}\\
%
	&
  \begin{array}{l}
  	\for{\ca{}} \for{(l_1 \composeL f, l_2 \composeL f) \in \amod{L}(\ca{})} \for{c, d} \\
  \hspace*{0.2cm} l_1 \composeL f \composeL c = l \composeL r \composeL d \;\land\; \left(\for{l'} l' \leq l_0 \land l' \leq l'_0 \implies l' = \unitL\right)  \;\implies\\
  \hspace*{0.4cm}\exsts{f', c'} (l_1 \composeL f', l_2 \composeL f') \in \amod{1}(\ca{}) \;\land\; l_1 \composeL f' \composeL c' =  l \composeL r \composeL d\\
		\hspace*{0.4cm}\lor\;l_2 \composeL f \composeL c \text{ is undefined}\\
		\hspace*{0.4cm}\lor\; \exsts{r'} l_2 \composeL f \composeL c = l \composeL r' \composeL d \;\land\; \extendsAMUpto{\amod{G}, \amod{L} \cup \amod{1}}{(m-1)}{l}{r'}{\amod{1}}
	\end{array}\label{L2:Goal2}
% 
\end{align}
%
%%
%
%
%
%
%
\textbf{RTS. (\ref{L2:Goal1})}\\
Pick an arbitrary $\ca{}, c, d, t, l_1, l_2, f, l_3, l_4$ such that 
\begin{align}
	&\left(\for{l'} l' \leq l_1 \land l' \leq l_2 \implies l' = \unitL\right)\;\land
	(l_1 \composeL f, l_2 \composeL f) \in \amod{1}(\ca{}) \label{L2:Ass19}\\
	&l_3 = l_1 \maxMeetL l \;\land\; l_1 = l_3 \composeL l_4 \;\land\; l = l_3 \composeL c \;\land\; r = l_4 \composeL d\label{L2:Ass20}\\
	&l_1 \composeL f \leq l \composeL r \composeL t\label{L2:Ass21}
%	& (l_3 \composeL c \composeL l_4 \composeL d, l_2 \composeL c \composeL d) \in \amod{}(\ca{}) \label{L2:Ass22}
\end{align}
%(\ref{L2:Ass})
From (\ref{L2:Ass1}), (\ref{L2:Ass4}), (\ref{L2:Ass19}), (\ref{L2:Ass21}) we know that 
%
\begin{align}
	\exsts{f'} (l_1 \composeL f', l_2 \composeL f') \in \amod{0}(\ca{}) \;\land\; l_1 \composeL f' \leq l \composeL r \composeL t \label{L2:Ass23}
\end{align}
%
From (\ref{L2:Ass5}), (\ref{L2:Ass20}) and (\ref{L2:Ass23}) we have:
%
\begin{align}
	\begin{array}{l l}
		&\extendsAMUpto{\amod{}, \amod{L}}{(n-1)}{l_2 \composeL c}{d}{\amod{0}} \;\land\\
		& t = \unitL \implies (l_1 \composeL c \composeL d, l_2 \composeL c \composeL d) \in \amod{}(\ca{}) \;\lor\; l_2 \composeL c \composeL d \hspace*{0.2cm}\text{ is undefined}
	\end{array} \label{L2:Ass24}
\end{align}
%(\ref{L2:Ass})
From (\ref{L2:Ass1}), (\ref{L2:Ass2}), (\ref{L2:Ass19})-(\ref{L2:Ass21}), (\ref{L2:Ass23}) and by definition of $\fences$ we have:
\begin{align}
	l_2 \composeL c \in F \label{L2:Ass25}
\end{align}
From (\ref{L2:Ass1}), (\ref{L2:Ass2}), (\ref{L2:Ass4}), (\ref{L2:Ass25}) and (\ref{L2:I.H}), we can rewrite (\ref{L2:Ass24}) as:
%
\begin{align}
	\begin{array}{l l}
		&\extendsAMUpto{\amod{}, \amod{L} \cup \amod{1}}{(n-1)}{l_2 \composeL c}{d}{\amod{1}} \;\land\\
		& t = \unitL \implies (l_1 \composeL c \composeL d, l_2 \composeL c \composeL d) \in \amod{}(\ca{}) \;\lor\; l_2 \composeL c \composeL d \hspace*{0.2cm}\text{ is undefined}
	\end{array} \label{L2:DismissedGoal4}
\end{align}\\\\
%
%
%
%
%
\noindent\textbf{RTS. (\ref{L2:Goal2})}\\
Pick an arbitrary $\ca{}, l_1, l_2, f, c, d$ such that:
%
\begin{align}
	\begin{array}{l}
		l_1 \composeL f \composeL c=  l \composeL r \composeL d\\
  	(l_1 \composeL f, l_2 \composeL f) \in \amod{L}(\ca{}) \\
  	\left(\for{l'} l' \leq l_1 \land l' \leq l_2 \implies l' = \unitL\right)\\
	\end{array} \label{LIH: Ass1}
\end{align} 
%
If $\amod{L} = \amod{1}$ the desired result holds trivially. On the other hand if $\amod{L} \not= \amod{1}$, then from (\ref{L2:Ass5}) we have:
\begin{align}
	\begin{array}{l}
		\exsts{f', c'} (l_1 \composeL f', l_2 \composeL f') \in \amod{0}(\ca{}) \;\land\; l_1 \composeL f' \composeL c' =  l \composeL r \composeL d\\
		\lor\;l_2 \composeL f \composeL c \text{ is undefined}\\
		\lor\; \exsts{r'} l_2 \composeL f \composeL c = l \composeL r' \composeL d \;\land\; \extendsAMUpto{\amod{G}, \amod{L}}{(m-1)}{l}{r'}{\amod{0}}
	\end{array} \nonumber
\end{align}
%
There are two cases to consider.\\

\noindent\textbf{Case 1.} 
%
\[
\begin{array}{l}
	l_2 \composeL f \composeL c \text{ is undefined}\\
	\lor\; \exsts{r'} l_2 \composeL f \composeL c = l \composeL r' \composeL d \;\land\;  \extendsAMUpto{\amod{G}, \amod{L}}{(m-1)}{l}{r'}{\amod{0}}
\end{array}
\]
%
From (\ref{L2:Ass1}), (\ref{L2:Ass2}), (\ref{L2:Ass4}) and (\ref{L2:I.H}) we can rewrite the above as:
%
\begin{align}
\begin{array}{l}
	l_2 \composeL f \composeL c \text{ is undefined}\\
	\lor\; \exsts{r'} l_2 \composeL f \composeL c = l \composeL r' \composeL d \;\land\; \extendsAMUpto{\amod{G}, \amod{L} \cup \amod{1}}{(m-1)}{l}{r'}{\amod{1}}
\end{array}\label{L2:Case1}
\end{align}\\

%
%
%
%
\noindent\textbf{Case 2.} 
%
\[
\begin{array}{l}
		\exsts{f', c'} (l_1 \composeL f',\ l_2 \composeL f') \in \amod{0}(\ca{}) \;\land\; l_1 \composeL f' \composeL c' = l \composeL r \composeL d
\end{array}
\]
%
Since $l_1 \composeL f' \leq l \composeL r \composeL d$, from (\ref{L2:Ass1}), (\ref{L2:Ass4}) and assumption of case 2 ($(l_1 \composeL f', l_2  \composeL f') \in \amod{0}(\ca{})$)  we can deduce:
%(\ref{L2:Ass})
\begin{align}
\begin{array}{l}
	\exsts{f''} (l_1 \composeL f'', l_2 \composeL f'') \in \amod{1}(\ca{}) \;\land\; l_1 \composeL f'' \leq l \composeL r \composeL d\\
	\lor\; \for{w \in (l \meetL l_1)} w \leq l_2
\end{array} \nonumber
\end{align}
%
There are two cases to consider:\\

\noindent\textbf{Case 2.1} 
%
%
\[
\begin{array}{l}
	\for{w \in \left(l \meetL l_1 \right)} w \leq l_2 
\end{array}
\]
%(\ref{L2:Ass})
Since $l_1 \leq l \composeL r \composeL d$, we know from lemma \ref{lem:nonEmptyOverlap} that $l \meetL l_1 \not= \emptyset$. Let $m = l_1 \maxMeetL l$. Then from the assumption of case 2.1. we know that $m \leq l_2$. On the other hand since $m \leq l_1$ and $m \leq l_2$, from (\ref{LIH: Ass1}) we have:
%
\begin{equation}
	m = l_1 \maxMeetL l = \unitL \nonumber
\end{equation} 
%
and thus
%
%
\begin{equation}
	l_1 \disjoint l  \label{L2:noOverlap}
\end{equation} 
%
%On the other hand, from (\ref{L2:noOverlap}), lemma \ref{lem:divideUpper} and since $l \composeL r \composeL d = l_1 \composeL f' \composeL c$ (assumption of case 2) and consequently, $l \leq l_1 \composeL f' \composeL c$, we have:
%%
%\begin{align}
%	\exsts{\h{}} l \composeL \h{} = f' \composeL c \nonumber
%\end{align}
%%
%and consequently, 
%%
%\begin{align}
%	l_2 \composeL f' \composeL c = l_2 \composeL l \composeL \h{} \nonumber
%\end{align}
%%
%That is
%%
%\begin{align}
%	\exsts{r'} l_2 \composeL f' \composeL c = l \composeL r' \label{L2:AssPart1}
%\end{align}
%%
%%(\ref{L2:Ass})
Since $\extendsAM{\amod{}, \amod{L}}{l}{r}{\amod{0}}$, we know $l_1 \composeL f \meetL l \composeL r = \emptyset \;\lor\; l_1 \leq l \composeL r$ and thus from assumption of case 2 we know $l_1 \leq l \composeL r$. Consequently, from (\ref{L2:noOverlap}) and lemma \ref{lem:divideUpper} we have:
%
\begin{align}
	\exsts{i} l_1 \composeL i = r \label{L2:AssResidue}
\end{align}
%
On the other hand, since $l \composeL r \composeL d = l_1 \composeL f' \composeL c$ (assumption of case 2), from (\ref{L2:AssResidue}) we know $l_1 \composeL f' \composeL c = l \composeL l_1 \composeL i \composeL d$ and consequently by cancellativity of separation algebras $f' \composeL c = l \composeL i \composeL d$ and thus
%
\begin{align}
	l_2 \composeL f' \composeL c = l_2 \composeL l \composeL i \composeL d \label{L2:AssPart1}
\end{align} 
%
Since $l_1 \composeL f' \leq l \composeL r \composeL d$ (assumption of case 2), from (\ref{L2:AssResidue}), (\ref{L2:noOverlap}) and assumption of case 2 we have:
%
\begin{align}
	& \extendsAMUpto{\amod{}, \amod{L}}{(n-1)}{l \composeL l_2}{i}{\amod{0}} \;\land \nonumber\\
	& d = \unitL \implies (l \composeL l_1 \composeL i, l \composeL l_2 \composeL i) \in \amod{}(\ca{}) \lor\; (l \composeL l_2 \composeL i) \text{ is undefined} \label{L2:Ass49}
\end{align} 
%
and consequently from Lemma  \ref{lemma:contextSwitch} we have:
%
\begin{align}
	& \extendsAMUpto{\amod{}, \amod{L}}{(n-1)}{l }{l_2 \composeL  i}{\amod{0}} \;\land\  \nonumber\\
	& d = \unitL \implies (l \composeL l_1 \composeL i, l \composeL l_2 \composeL i) \in \amod{}(\ca{}) \;\lor\; (l \composeL l_2 \composeL i) \text{ is undefined} \label{L2:Ass45}
\end{align} 
%
%(\ref{L2:Ass})
From (\ref{L2:Ass1})-(\ref{L2:Ass4}), (\ref{L2:Ass45}) and (\ref{L2:I.H}) we can rewrite (\ref{L2:Ass45}) as:
%(\ref{L2:Ass})
\begin{align}
	& \extendsAMUpto{\amod{}, \amod{L} \cup \amod{1}}{(n-1)}{l }{l_2 \composeL  i}{\amod{1}} \;\land \nonumber\\
	& d = \unitL \implies (l \composeL l_1 \composeL i, l \composeL l_2 \composeL i) \in \amod{}(\ca{}) \;\lor\; (l \composeL l_2 \composeL i) \text{ is undefined} \label{L2:Ass52}
\end{align}
%
and thus from (\ref{L2:AssPart1}) we have:
%
\begin{align}
	\exsts{r'}	l_2 \composeL f' \composeL c = l \composeL r' \composeL d \;\land\; \extendsAMUpto{\amod{}, \amod{L} \cup \{\amod{1}\}}{(n-1)}{l }{r'}{\amod{1}} \nonumber\\
	\lor\; (l \composeL l_2 \composeL i) \text{ is undefined}\label{L2:Case2.1}
\end{align}
%
%
%
%
%
\noindent\textbf{Case 2.2} 
%
\[
\begin{array}{l}
	\exsts{f''} (l_1 \composeL f'', l_2 \composeL f'') \in \amod{1}(\ca{}) \;\land\; l_1 \composeL f'' \leq l \composeL r \composeL d
\end{array}
\]
%(\ref{L2:Ass})
and consequently 
\begin{align}
\begin{array}{l}
	\exsts{f'', c} (l_1 \composeL f'',\ l_2 \composeL f'') \in \amod{1}(\ca{}) \;\land\; l_1 \composeL f'' \composeL c' = l \composeL r \composeL d
\end{array} \label{L2:Case2.2}
\end{align}
%
as required.
\end{proof}
\end{lemma}
%
%
\begin{lemma}[]
%
\[
		\fence{} \fences I \;\land\; I \weakenI{\fence{}} I_1 \implies \fence{} \fences I_1
\]
%
\begin{proof}
\todo
\end{proof}
\end{lemma}
%
%
\input{Soundness/amodMerge.tex}
\begin{lemma}[] \label{lem:extension}
%
\[
		P \containI I  \Rrightarrow \exsts{\capAss{1}, \capAss{2}} \;\; \capAss{1} * \shared{P * \capAss{2}}{I}
\]
%
\begin{proof}
\textbf{RTS. }
%
\[
\begin{array}{l}
	\for{\lenv} \for{w_1 \in \sem[\lenv]{P}} \exsts{w_2 \in \sem[\lenv]{\exsts{\capAss{1}} \;\; \capAss{1} * \shared{P * \capAss{2}}{I}}}\\
	\hspace*{1cm} (w_1, w_2) \in \guarantee \;\land\; \heapPart{\left(\collapseW{w_1}\right)} = \heapPart{\left(\collapseW{w_2}\right)}
\end{array}
\]
%
Pick an arbitrary $\lenv$, $w_1 = (l, s, \amod{}, \amod{L}) \in \sem[\lenv]{P}$ and set $K$ such that:
\begin{align}
%	K = 
%	\semK[\lenv]{\left( \bigvee\limits_{\lambda \vec{x}. \capAss{}: a \in \dom{I}} \capAss{}\right) \;\lor\; \capAss{1} }
%	\;\land\; K \disjoint \dom{\amod{L}} \label{LE:Ass1}
	K = 
	\semK[\lenv]{\capAss{1} \lor \capAss{2}}
	\;\land\; K \disjoint \dom{\amod{L}} \label{LE:Ass1}
\end{align}	 
%
Since $(l, s, \amod{}, \amod{L}) \in \sem[\lenv]{P}$, we know 
\begin{align}
	\exsts{\fence{L}} s \in \fence{L} \;\land\; \fence{L} \strictfences \amod{L} \label{LE:Ass2}
\end{align} 
%Pick arbitrary $l_1, \cdots, l_n \in \LStates$, $\amod{1} , \cdots, \amod{n} \in \AMods$, $F_1, \cdots, F_n \in \pset{\LStates}$ such that 
%%
%\begin{align}
%\begin{array}{l}
%	l_1 \composeL \cdots \composeL l_n = s \\
%	\for{\amod{i}, \amod{j} \in \left(\amod{1} \cup \cdots \cup \amod{n}\right)} \dom{\amod{i}} \disjoint \dom{\amod{j}}\\
%	\dom{\amod{}} = \dom{\amod{1}} \cup \cdots \cup \dom{\amod{n}}\\
%	\for{i \in 1, \cdots, n} l_i \in F_i \;\land\; F_i \strictfences \amod{i}\;\land\;\\
%	\hspace*{1cm}\extendsAM{\amod{}}{l_i}{l_1 \composeL \cdots \composeL l_{i-1} \composeL l_{i+1} \composeL \cdots \composeL l_n}{\amod{i}} \label{LE:Ass2}
%\end{array}
%\end{align}
%%
On the other hand, from the premise of the lemma we know 
%
\begin{align}
	\exsts{\fence{}} l \in \fence{} \;\land\; \fence{} \strictfences \semI[\lenv]{I} \label{LE:Ass3}
\end{align}
%(\ref{LE:Ass})
Since $\wf{l, s, \amod{}, \amod{L}}$, we know $l \composeL s \text{ is defined}$ and thus from (\ref{LE:Ass1})-(\ref{LE:Ass3}) and lemma \ref{lem:amodWitness} we know:
%
\begin{align}
\begin{array}{l}
	\exsts{\amod{}', \fence{}'} l \composeL s \in \fence{}' \;\land\; \fence{}' \strictfences \amod{L} \cup \semI[\lenv]{I} \;\land\; \extendsAM{\amod{}', \amod{L} \cup \semI[\lenv]{I}}{l}{s}{\semI[\lenv]{I}} \;\land\\
	\hspace*{1.3cm}\for{l', r'} \for{\amod{1} \subseteq \amod{L}} l' \composeL r' = s \;\land\; \extendsAM{\amod{}, \amod{L}}{l'}{r'}{\amod{1}} \implies\\
	\hspace*{1.8cm}\extendsAM{\amod{}', \amod{L} \cup \semI[\lenv]{I}}{l'}{r' \composeL l}{\amod{1}} 
\end{array}\label{LE:Ass4}
\end{align}
%
%Pick $\amod{}'$ such that (\ref{LE:Ass4}) is satisfied. Then from (\ref{LE:Ass2}) and (\ref{LE:Ass4}) we know
%%
%\begin{align}
%	\expandsAM{\amod{}'}{s}{l}{\amod{}} \;\land\; \extendsAM{\amod{}'}{l}{s}{\intermediateSemI{I}} \label{LE:Ass5}
%\end{align}
%%
Pick $\amod{}'$ such that (\ref{LE:Ass4}) is satisfied. Pick $\ca{1} \in \semK[\lenv]{\capAss{1}}$, $\ca{2} \in \semK[\lenv]{\capAss{2}}$ and $w_2 = ( (\unitH, \ca{1}), l \composeL s \composeL (\unitH, \ca{2}), \amod{}', \amod{L} \cup \intermediateSemI{I} )$. Then from (\ref{LE:Ass1}) and (\ref{LE:Ass4}) we know
%
\begin{align}
	(w_1, w_2) \in \guarantee \label{LE:Ass6}
\end{align}
%
On the other hand, from the definition of $\collapseW{.}$ we know:
%(\ref{LE:Ass})
\begin{align}
	\heapPart{\left(\collapseW{w_1}\right)} = \heapPart{\left(\collapseW{w_2}\right)} \label{LE:Ass7}
\end{align}
%
Finally since $w_2 \in \sem[\lenv]{\capAss{1} * \shared{P * \capAss{2}}{I}}$, from (\ref{LE:Ass6}) and (\ref{LE:Ass7}) we have
%
\begin{align}
	(w_1, w_2) \in \guarantee \;\land\; \heapPart{\left(\collapseW{w_1}\right)} = \heapPart{\left(\collapseW{w_2}\right)}
\end{align}
%
as required.
\end{proof}
\end{lemma}
%
%
\input{Soundness/amodConstruction.tex}
%
%
\begin{lemma}[]\label{lem:nonEmptyOverlap}
%
\[
	\for{a, b, c \in \LStates} a \leq b \composeL c \implies a \meetL b \not= \emptyset
\]
%
\begin{proof} By contradiction.
Take arbitrary $a, b, c \in \LStates$ such that 
%
\begin{equation}
	a \leq b \composeL c \label{L5:Ass1}
\end{equation}
%
and assume
%
\begin{equation}
	a \meetL b = \emptyset \label{L5:Ass2}
\end{equation}
%
From (\ref{L5:Ass2}) and by definition of $\meetL$, we have:
%
\begin{equation}
	\neg\exsts{d, e, f, g} a = d \composeL e \;\land\; b = e \composeL f \;\land\; d \composeL e \composeL f = g \label{L5:Ass3}
\end{equation}
%
From (\ref{L5:Ass1}) we have $\exsts{h} a \composeL h = b \composeL c$ and consequently by the cross-splittability property we have:
%
\begin{align}
	\exsts{ab, ac, hb, hc, t} \hspace*{2cm}&
	ab \composeL ac = a 	\label{L5:Ass4}\\
	& hb \composeL hc = h \label{L5:Ass5}\\
	& ab \composeL hb = b \label{L5:Ass6}\\
	& ac \composeL hc = c \label{L5:Ass7}\\
	& t = ab \composeL ac \composeL hb \composeL hc \label{L5:Ass8}
\end{align}
%
From (\ref{L5:Ass8}) we have:
%
\begin{equation}
	\exsts{s} ab \composeL ac \composeL hb = s \label{L5:Ass9}
\end{equation}
%
From (\ref{L5:Ass4}), (\ref{L5:Ass6}) and (\ref{L5:Ass9}) we have: 
%
\begin{equation}
	\exsts{d, e, f, g} a = d \composeL e \;\land\; b = e \composeL f \;\land\; d \composeL e \composeL f = g \label{L5:Ass10}
\end{equation}
%
From (\ref{L5:Ass3}) and (\ref{L5:Ass10}) we derive a contradiction and can hence deduce:
%
\begin{equation}
	a \meetL b \not= \emptyset \nonumber
\end{equation}
%
as required.
\end{proof}
\end{lemma}
%
%
\begin{lemma}[]\label{lem:divideUpper}
%
Given any separation algebra ($\mathcal{M}, \compose{\mathcal{M}}, \unit{\mathcal{M}}$) with the cross-split property:
\[
	\for{a, b, c \in \mathcal{M}} a \leq b \compose{\mathcal{M}} c \implies \exsts{m, n} a = m \compose{\mathcal{M}} n \;\land\; m \leq b \;\land\; n \leq c
\]
%
\begin{proof}
Pick an arbitrary $a, b, c \in \mathcal{M}$. Since $a \leq b \compose{\mathcal{M}} c$, we know $\exsts{d \in \mathcal{M}}$ such that:
%
\begin{equation}
	a \compose{\mathcal{M}} d = b \compose{\mathcal{M}} c \label{L6:Ass1}
\end{equation}
%
By the cross-split property of $\mathcal{M}$, We can deduce: $\exsts{ab, ac, db, dc \in \mathcal{M}}$ such that:
%
\begin{align}
	a = ab \compose{\mathcal{M}} ac \label{L6:Ass2}\\
	b = ab \compose{\mathcal{M}} db \label{L6:Ass3}\\
	c = ac \compose{\mathcal{M}} dc \label{L6:Ass4}\\
	d = db \compose{\mathcal{M}} dc \nonumber 
\end{align}
%
Since $ab \leq b$ (\ref{L6:Ass3}) and $ac \leq c$ (\ref{L6:Ass4}), from (\ref{L6:Ass2}) we can deduce:
%
\begin{equation}
	\exsts{m, n \in \mathcal{M}} a = m \compose{\mathcal{M}} n \;\land\; m \leq b \;\land\; n \leq c \nonumber
\end{equation}
%
as required.
\end{proof}
\end{lemma}
%
%
\begin{lemma}[]\label{lem:disjointByOrder}
Given any separation algebra ($\mathcal{M}, \compose{\mathcal{M}}, \unit{\mathcal{M}}$),
\[
	\for{a, b, c, d \in \mathcal{M}} a \compose{\mathcal{M}} b = d \;\land\; c \leq b \implies 
	\exsts{f \in \mathcal{M}} a \compose{\mathcal{M}} c = f
\]
%
\begin{proof}
Pick an arbitrary $a, b, c, d \in \mathcal{M}$ such that:
%
\begin{align}
	a \compose{\mathcal{M}} b = d \label{L7:Ass1}\\
	c \leq b \label{L7:Ass2}
\end{align}
%
From (\ref{L7:Ass2}), we have: 
%
\begin{equation}
	\exsts{e \in \mathcal{M}} c \compose{\mathcal{M}} e = b \label{L7:Ass3}
\end{equation}
%
and consequently from (\ref{L7:Ass1}) we have:
%
\begin{equation}
	a \compose{\mathcal{M}} c \compose{\mathcal{M}} e = d \label{L7:Ass4}
\end{equation}
%
Since $e \leq d$ (\ref{L7:Ass4}), we have: 
%
\begin{equation}
	\exsts{f \in \mathcal{M}} e \compose{\mathcal{M}} f = d \label{L7:Ass5}
\end{equation} 
%
From (\ref{L7:Ass4}), (\ref{L7:Ass5}) and cancellativity of separation algebras we have:
%
\begin{equation}
	a \compose{\mathcal{M}} c = f
\end{equation}
%
and thus
%
\begin{equation}
	\exsts{f \in \mathcal{M}} a \compose{\mathcal{M}} c = f
\end{equation}
%
as required.
\end{proof}
\end{lemma}
%
%
\begin{lemma}[]\label{lem:amodClosureImplication}
For all $l, r \in \LStates$, $\amod{}, \amod{L}, \amod{}' \in \AMods$ and $n \in \NatsPlus$
%
\[
	\extendsAMUpto{\amod{}, \amod{L}}{n}{l}{r}{\amod{}'} \implies \extendsAMUpto{\amod{}, \amod{L}}{(n-1)}{l}{r}{\amod{}'}
\]
%
\begin{proof} By induction on number of steps $n$.\\
Pick an arbitrary $l, r \in \LStates$, $\amod{}, \amod{L}, \amod{}' \in \AMods$ and $n \in \NatsPlus$.\\
\textbf{Base case: n = 1}\\
\textbf{RTS.} 
%
\begin{equation}
	\extendsAMUpto{\amod{}, \amod{L}}{0}{l}{r}{\amod{}'} \nonumber
\end{equation}
%
This holds trivially by definition of $\left(\amod{}, \amod{L}\right)\!\downarrow_{0}$\\

\noindent\textbf{Inductive case}\\
\textbf{Assume:}
%
\begin{align}
	\extendsAMUpto{\amod{}, \amod{L}}{(n+1)}{l}{r}{\amod{}'} \label{L9:Ass1}\\
	\extendsAMUpto{\amod{}, \amod{L}}{n}{l}{r}{\amod{}'} \implies \extendsAMUpto{\amod{}}{(n-1)}{l}{r}{\amod{}'} \tag{I.H} \label{L9:I.H}
\end{align}
%
\textbf{Show:}
%
\begin{align}
	&\begin{array}{l}
			\for{\ca{}, c, d, t, l_3, l_4} \for{(l_1 \composeL f, l_2 \composeL f) \in \amod{}'(\ca{})} \\
%			
			\hspace*{0.2cm}\left(\for{l'} l' \leq l_1 \;\land\; l' \leq l_2 \implies l' = \unitL \right) \;\land\; l_1 \composeL f \leq l \composeL r \composeL t \;\land\\
%			
			\hspace*{0.2cm} l_1 = l_3 \composeL l_4 \;\land\; 	l_1 \maxMeetL l = l_3 \;\land\; l = l_3 \composeL c \;\land\; r = l_4 \composeL d \implies \\
%			
			\hspace*{0.5cm}\extendsAMUpto{\amod{}, \amod{L}}{(n-1)}{l_2 \composeL c}{d}{\amod{}'} \;\land\\
			\hspace*{0.5cm} t = \unitL \implies (l_1 \composeL c \composeL d, l_2 \composeL c \composeL d) \in \amod{}(\ca{}) 
			\;\lor\; l_2 \composeL c \composeL d \text{ is undefined} 	
	\end{array}\label{L9:Goal1}\\
%
  &\begin{array}{l}
  	\for{\ca{}} \for{(l_1 \composeL f, l_2 \composeL f) \in \amod{L}(\ca{})} \for{c, d} \\
  \hspace*{0.2cm} l_1 \composeL f \composeL c = l \composeL r \composeL d \;\land\; \left(\for{l'} l' \leq l_0 \land l' \leq l'_0 \implies l' = \unitL\right)  \;\implies\\
  \hspace*{0.4cm}\exsts{f', c'} (l_1 \composeL f', l_2 \composeL f') \in \amod{}'(\ca{}) \;\land\; l_1 \composeL f' \composeL c' =  l \composeL r \composeL d\\
		\hspace*{0.4cm}\lor\;l_2 \composeL f \composeL c \text{ is undefined}\\
		\hspace*{0.4cm}\lor\; l_1 \maxMeetL l = \unitL \;\land\; \exsts{r'} l_2 \composeL f \composeL c = l \composeL r' \composeL d \;\land\; \extendsAMUpto{\amod{}, \amod{L}}{(n-1)}{l}{r'}{\amod{}'}
  \end{array} \label{L9:Goal2}
\end{align}
%

\noindent\textbf{RTS. (\ref{L9:Goal1})}\\
Pick an arbitrary $\ca{}, c, d, t, l_1, l_2, l_3, l_4, f$ such that
%
\begin{equation}
\hspace*{-0.15cm}
\begin{array}{l}
	(l_1 \composeL f, l_2 \composeL f) \in \amod{}'(\ca{}) \;\land\; 
	\left(\for{l'} l' \leq l_1 \land l' \leq l_2 \implies l' = \unitL \right)
	\;\land\; l_1 \composeL f \leq l \composeL r \composeL t\\
%
	\land\; l_1 = l_3 \composeL l_4 \;\land\; 	l_1 \maxMeetL l = l_3 \;\land\; l = l_3 \composeL c \;\land\; r = l_4 \composeL d
\end{array} \label{L9:Ass2}
\end{equation}
%
From (\ref{L9:Ass1}) and (\ref{L9:Ass2}) we have:
%
\begin{align}
	& \extendsAMUpto{\amod{}, \amod{L}}{n}{l_2 \composeL c}{d}{\amod{}'} \nonumber \;\land\\
	& t = \unitL \implies (l_1 \composeL c \composeL d, l_2 \composeL c \composeL d) \in \amod{}(\ca{}) \;\lor\; l_2 \composeL c \composeL d \text{ is undefined} \nonumber
\end{align}
%
From (\ref{L9:I.H}) we can rewrite the above as 
%
\begin{align}
	& \extendsAMUpto{\amod{}, \amod{L}}{(n-1)}{l_2 \composeL c}{d}{\amod{}'} \nonumber \;\land\\
	& t = \unitL \implies (l_1 \composeL c \composeL d, l_2 \composeL c \composeL d) \in \amod{}(\ca{}) \;\lor\; l_2 \composeL c \composeL d \text{ is undefined} \label{L9:Ass3}
\end{align}
%
as required.\\

\noindent\textbf{RTS. (\ref{L9:Goal2})}\\
Pick an arbitrary $\ca{}, l_1, l_2, f, c, d$ such that
%
\begin{align}
	\begin{array}{l}
		(l_1 \composeL f, l_2 \composeL f) \in \amod{L}(\ca{})\\
  	l_1 \composeL f \composeL c = l \composeL r \composeL d\\
  	\for{l'} l' \leq l_0 \land l' \leq l'_0 \implies l' = \unitL
	\end{array} \label{L9:Ass4}
\end{align}
%
From (\ref{L9:Ass1}) and (\ref{L9:Ass4}) we have:
%
\begin{align}
  \begin{array}{l}
  	\exsts{f', c'} (l_1 \composeL f', l_2 \composeL f') \in \amod{}'(\ca{}) \;\land\; l_1 \composeL f' \composeL c' =  l \composeL r \composeL d\\
		\lor\;l_2 \composeL f \composeL c \text{ is undefined}\\
		\lor\; l_1 \maxMeetL l = \unitL \;\land\; \exsts{r'} l_2 \composeL f \composeL c = l \composeL r' \composeL d \;\land\; \extendsAMUpto{\amod{}, \amod{L}}{n}{l}{r'}{\amod{}'}
  \end{array}\label{L9:Ass5}
\end{align}
%
From (\ref{L9:I.H}) we can rewrite (\ref{L9:Ass5}) as
%
\begin{align}
	\begin{array}{l}
  	\exsts{f', c'} (l_1 \composeL f', l_2 \composeL f') \in \amod{}'(\ca{}) \;\land\; l_1 \composeL f' \composeL c' =  l \composeL r \composeL d\\
		\lor\;l_2 \composeL f \composeL c \text{ is undefined}\\
		\lor\; l_1 \maxMeetL l = \unitL \;\land\; \exsts{r'} l_2 \composeL f \composeL c = l \composeL r' \composeL d \;\land\; \extendsAMUpto{\amod{}, \amod{L}}{n}{l}{r'}{\amod{}'}
  \end{array} \nonumber
\end{align}
%
as required.
\end{proof}
\end{lemma}
%
%
%\begin{lemma}[]\label{lem:noMeetByOrder}
%Given any separation algebra ($\mathcal{M}, \compose{\mathcal{M}}, \unit{\mathcal{M}}$) with the cross-split property,
%\[
%\begin{array}{l}
%	\for{a, b, c, d \in \mathcal{M}} a \meet{\mathcal{M}} b = \emptyset \;\land\; a \leq d \;\land\; b \leq c \implies \\
%	\hspace*{1cm} c \meet{\mathcal{M}} d = \emptyset
%\end{array}
%\]
%%
%\begin{proof}
%\todo
%\end{proof}
%\end{lemma}
%%
%


