\newpage
\section*{Soundness}
\begin{lemma}[Atomic Command Soundness]
For all $\atom{} \in \Atoms$, $\left(W_1, \atom{}, W_2\right) \in \AxiomsA$ and $w \in \Worlds$:
%
\[
	\opSemA{\atom{}}{\reifyW{W_1 \composeW \{w\}}} \subseteq \reifyW{W_2 \composeH \rely\left(\{w\}\right)}
\]
%
\begin{proof}
By induction over the structure of \atom{}.\\

\noindent\textbf{Case \hspace*{0.3cm}}$\atomic{\seq{}}$\\
Pick an arbitrary $\seq{} \in \Seqs$ and $w \in \Worlds$.\\
\textbf{RTS.}
%
\[
	\opSemA{\atomic{\seq{}}}{\reifyW{W_1 \composeW \{w\}}} \subseteq \reifyW{W_2 \composeH \rely\left(\{w\}\right)}
\]
%
where
%
\begin{align}
	\left\{
	\hspace*{-0.15cm}
	\begin{array}{l | l}
		 \left(W_1, \atomic{\seq{}}, W_2 \right) &
		 (\Hp{1}, \seq{}, \Hp{2}) \in \AxiomsSeq \;\land\; \repartitions{W_1}{W_2}{\Hp{1}}{\Hp{2}}
	\end{array}
	\hspace*{-0.15cm}
	\right\}
	\subset \AxiomsA
	\nonumber
\end{align}
%
\begin{proof}
By calculation.\\
%
\[
\begin{array}{r l}
	\opSemA{\atomic{\seq{}}}{\reifyW{W_1 \composeW \{w\}}} &
	= 
	\left\{
	\hspace*{-0.15cm}
	\begin{array}{l | l}
		\reifyW{\left(l \composeL \localPart{w}, g, \lmod, \gmod \right)}
		&
		\begin{array}{l}
			(l, g, \lmod, \gmod) \in W_1 \;\land\\ 
			(\Hp{1}, \seq{}, \Hp{2}) \in \AxiomsSeq \\
			\land\;\repartitions{W_1}{W_2}{\Hp{1}}{\Hp{2}}
		\end{array}			
	\end{array}
	\hspace*{-0.15cm}
	\right\}\\
	

	
	\left(\text{def. of } \reifyW{.}	\right)
	& =
	\left\{
	\hspace*{-0.15cm}
	\begin{array}{l | l}
		\reifyH{\heapPart{l} \composeH \heapPart{g} \composeH \heapPart{\left(\localPart{w}\right)}}
		&
		\hspace*{-0.15cm}
		\begin{array}{l}
			(l, g, \lmod, \gmod) \in W_1 \;\land\\ 
			(\Hp{1}, \seq{}, \Hp{2}) \in \AxiomsSeq \\
			\land\;\repartitions{W_1}{W_2}{\Hp{1}}{\Hp{2}}
		\end{array}			
		\hspace*{-0.15cm}
	\end{array}
	\hspace*{-0.15cm}
	\right\}\\
	
	
	\left(\text{def. of } \Rrightarrow	\right)
	& =
	\left\{
	\hspace*{-0.15cm}
	\begin{array}{l | l}
		\reifyH{\h{1} \composeH \h{}' \composeH \heapPart{\left(\localPart{w}\right)}}
		&
		\hspace*{-0.15cm}
		\begin{array}{l}
			(l, g, \lmod, \gmod) \in W_1 \;\land\\ 
			(\Hp{1}, \seq{}, \Hp{2}) \in \AxiomsSeq \\
			\land\;\repartitions{W_1}{W_2}{\Hp{1}}{\Hp{2}}\\
			\land\; \h{1} \composeH \h{}' = \heapPart{l} \composeH \heapPart{s}\\
			\land\; \h{1} \in \Hp{1}
		\end{array}			
		\hspace*{-0.15cm}
	\end{array}
	\hspace*{-0.15cm}
	\right\}\\
	
	
	\left(\text{Lemma } \ref{lem:seqSoundness} \right)
	& \subseteq
	\left\{
	\hspace*{-0.15cm}
	\begin{array}{l | l}
%		\reifyH{\heapPart{l} \composeH \heapPart{g} \composeH \heapPart{\left(\localPart{w}\right)}}
		\reifyH{\h{2} \composeH \h{}' \composeH \heapPart{\left(\localPart{w}\right)}}
		&
		\hspace*{-0.15cm}
		\begin{array}{l}
			(l, g, \lmod, \gmod) \in W_1 \;\land\\ 
			(\Hp{1}, \seq{}, \Hp{2}) \in \AxiomsSeq \\
			\land\;\repartitions{W_1}{W_2}{\Hp{1}}{\Hp{2}}\\
			\land\; \h{1} \composeH \h{}' = \heapPart{l} \composeH \heapPart{g}\\
			\land\; \h{1} \in \Hp{1} \;\land\; \h{2} \in \Hp{2}
		\end{array}			
		\hspace*{-0.15cm}
	\end{array}
	\hspace*{-0.15cm}
	\right\}\\
	
	
	
	\left(\text{def. of } \Rrightarrow \right)
	& =
	\left\{
	\hspace*{-0.15cm}
	\begin{array}{l | l}
%		\reifyH{\heapPart{l} \composeH \heapPart{s} \composeH \heapPart{\left(\localPart{w}\right)}}
		\reifyH{ \heapPart{\left(\collapseW{w_2}\right)}  \composeH \heapPart{\left(\localPart{w}\right)}}
		&
		\hspace*{-0.15cm}
		\begin{array}{l}
			(l, g, \lmod, \gmod) \in W_1 \;\land\\ 
			(\Hp{1}, \seq{}, \Hp{2}) \in \AxiomsSeq \\
			\land\;\repartitions{W_1}{W_2}{\Hp{1}}{\Hp{2}}\\
			\land\; w_2 \in W_2\\
			\land\; \left(\;(l, g, \lmod{}, \gmod), w_2 \right) \in \guarantee
		\end{array}			
		\hspace*{-0.15cm}
	\end{array}
	\hspace*{-0.15cm}
	\right\}\\
	
	
	
	\left(\text{def. of } \reifyW{.} \right)
	& =
	\left\{
	\hspace*{-0.15cm}
	\begin{array}{l | l}
		\reifyW{\left(l' \composeL \localPart{w}, g', \lmod', \gmod' \right)}
		&
		\hspace*{-0.15cm}
		\begin{array}{l}
			(l, g, \lmod, \gmod) \in W_1 \;\land\\ 
			\land\;(l', g', \lmod', \gmod') \in W_2\\
			\land\; \left(\;(l, g, \lmod, \amod{L}), (l', g', \lmod', \gmod') \right) \in \guarantee
		\end{array}			
		\hspace*{-0.15cm}
	\end{array}
	\hspace*{-0.15cm}
	\right\}\\
	
	
	
	\left(\text{Lemma } \ref{lem:guaranteeContainment} \right)
	& 
	\subseteq	\reifyW{W_2 \composeW \rely\left( \{w\} \right)}

	
\end{array}
\]
%
as required.
\end{proof}
\renewcommand{\qed}{}
\end{proof}
\end{lemma}
%
%
\begin{lemma}[\forgetRule]
%
\[
	\shared{P \sepish Q}{I} \implies \shared{P}{I}
\]
%
\textbf{RTS.} $\for{\lenv\in \LEnv} \left\{w \mid w, \lenv |= \shared{P \sepish Q}{I}\right\} \subseteq \left\{w \mid w, \lenv |= \shared{P}{I} \right\}$
%
\begin{proof}
\[
\begin{array}{r l}
	\left\{w \mid w, \lenv |= \shared{P \sepish Q}{I}\right\} &
	= \left\{
	\hspace*{-0.2cm}
	\begin{array}{l | l}
		\left(
		\hspace*{-0.15cm}
		\begin{array}{l}
		(\unitL, \\
		(p \composeL c \composeL q \composeL r)\\
		, \lmod, \gmod
		\end{array}
		\hspace*{-0.15cm}
		\right)
		&
		\hspace*{-0.1cm}
		\begin{array}{l}

			(p \composeL c), \lenv |=_{(p \composeL c \composeL q \composeL r), \lmod, \gmod} P \\
			\land (q \composeL c), \lenv |=_{(p \composeL c \composeL q \composeL r), \lmod, \gmod} Q \\
			
			\land r \in \LStates \\
			
			\land \extendsAM{\lmod, \gmod}{p \composeL c \composeL q}{r}{\semI[\lenv]{I}}
		\end{array}
		\hspace*{-0.1cm}
	\end{array}
	\hspace*{-0.2cm}
	\right\} \\
	
	
	
	\text{By Lemma \ref{lemma:contextSwitch}} & 
	\subseteq \left\{
	\hspace*{-0.2cm}
	\begin{array}{l | l}
		\left(
		\hspace*{-0.15cm}
		\begin{array}{l}
		(\unitL, \\
		(p \composeL c \composeL q \composeL r)\\
		, \lmod{}, \gmod
		\end{array}
		\hspace*{-0.15cm}
		\right)
		&
		\hspace*{-0.1cm}
		\begin{array}{l}
			(p \composeL c), \lenv |=_{(p \composeL c \composeL q \composeL r), \lmod, \gmod} P \\
			\land (q \composeL c), \lenv |=_{(p \composeL c \composeL q \composeL r), \lmod, \gmod} Q \\
			
			\land r \in \LStates \;\;\land\\
			
			\land \extendsAM{\lmod{}, \gmod}{p \composeL c}{\ q \composeL r}{\semI[\lenv]{I}}
		\end{array}
		\hspace*{-0.1cm}
	\end{array}
	\hspace*{-0.2cm}
	\right\} \\
	
	
	
	
	
	
	& \subseteq
	\left\{
	\hspace*{-0.2cm}
	\begin{array}{l | l}
		\left(
		\hspace*{-0.15cm}
		\begin{array}{l}
		(\unitL, \\
		(p \composeL r)\\
		, \lmod{}, \gmod
		\end{array}
		\hspace*{-0.15cm}
		\right)
		&
		\hspace*{-0.1cm}
		\begin{array}{l}

			p, \lenv |=_{(p \composeL r), \lmod, \gmod} P \\
			\land r \in \LStates 
			\land \extendsAM{\lmod{}, \gmod}{p}{\ r}{\semI[\lenv]{I}}
		\end{array}
		\hspace*{-0.1cm}
	\end{array}
	\hspace*{-0.2cm}
	\right\} \\
	
	
	& = \left\{ w \mid w, \lenv |= \shared{P}{I}\right\}
\end{array}
\]
%
as required.
\end{proof}
%
\end{lemma}
%%
%%
%\begin{lemma}[Interference Hiding]
%%
%\[
%	\shared{P}{I}^{\ \fence{}} \;\land\; I \weakenI{\fence{}} I_1 \;\semimplies\;\; \shared{P}{I_1}
%\]
%%
%\textbf{RTS.} 
%\[
%\begin{array}{l}
%	\for{\lenv} 
%		\fence{} \fences \left(\intermediateSemI{I}, \semL[\lenv]{P}\right) 
%		\;\land\; 
%		\intermediateSemI{I} \weakenI{\fence{}} \intermediateSemI{I_1} 
%		\semimplies\\
%	  \hspace*{2cm}\sem[\lenv]{\shared{P}{I}} \subseteq  \sem[\lenv]{\shared{P}{I_1}}
%\end{array}
%\]
%%
%\begin{proof}
%\[
%\begin{array}{r l}
%	\sem[\lenv]{\shared{P}{I}} &
%	= \left\{
%	\hspace*{-0.2cm}
%	\begin{array}{l | l}
%		\left(
%		\hspace*{-0.15cm}
%		\begin{array}{l}
%		\unitL,
%		(p \composeL r)
%		, \amod{}
%		\end{array}
%		\hspace*{-0.15cm}
%		\right)
%		&
%		\hspace*{-0.1cm}
%		\begin{array}{l}
%			\left(
%			\hspace*{-0.15cm}
%			\begin{array}{l}
%			p, 
%			(p \composeL r)
%			, \amod{}
%			\end{array}
%			\hspace*{-0.15cm}
%			\right) \in \sem[\lenv]{P}\\
%			
%
%			
%			\land\; r \in \LStates \;\;\land\;\; \intermediateSemI{I} = \amod{}'\\
%			
%			\extendsAM{\amod{}}{p}{\ r}{\ \amod{}'}
%		\end{array}
%		\hspace*{-0.1cm}
%	\end{array}
%	\hspace*{-0.2cm}
%	\right\} \\
%	
%	
%	
%	\text{By Lemma \ref{lem:amodHiding}} & 
%	\subseteq \left\{
%	\hspace*{-0.2cm}
%	\begin{array}{l | l}
%		\left(
%		\hspace*{-0.15cm}
%		\begin{array}{l}
%		\unitL,
%		(p \composeL r)
%		, \amod{}
%		\end{array}
%		\hspace*{-0.15cm}
%		\right)
%		&
%		\hspace*{-0.1cm}
%		\begin{array}{l}
%			\left(
%			\hspace*{-0.15cm}
%			\begin{array}{l}
%			p, 
%			(p \composeL r)
%			, \amod{}
%			\end{array}
%			\hspace*{-0.15cm}
%			\right) \in \sem[\lenv]{P}\\
%			
%
%			
%			\land\; r \in \LStates \;\;\land\;\; \intermediateSemI{I_1} = \amod{}'\\
%			
%			\extendsAM{\amod{}}{p}{\ r}{\ \amod{}'}
%		\end{array}
%		\hspace*{-0.1cm}
%	\end{array}
%	\hspace*{-0.2cm}
%	\right\} \\
%	
%	
%	
%	
%	
%	
%	
%	
%	& = \sem[\lenv]{\shared{P}{I_1}}
%\end{array}
%\]
%%
%\end{proof}
%%
%\end{lemma}
%%
%%
\begin{lemma}[\mergeRule]
%
\[
	\shared{P}{I_1} * \shared{Q}{I_2} \;\implies\;\; \shared{P \sepish Q}{I_1 \cup I_2}
\]
%
\textbf{RTS.} 
\[
\begin{array}{l l}
	\for{\lenv\in \LEnv} \left\{ w \mid w, \lenv |= \shared{P}{I_1} * \shared{Q}{I_2} \right\} \subseteq \left\{ w \mid w, \lenv |= \shared{P \sepish Q}{I_1 \cup I_2}\right\}
\end{array}
\]
%
\begin{proof}
\[
\begin{array}{r l}
	& \left\{ w \mid w, \lenv |= \shared{P}{I_1} * \shared{Q}{I_2} \right\}\\
	
	= &
	\left\{
	\hspace*{-0.2cm}
	\begin{array}{l | l}
		\left(
		\hspace*{-0.15cm}
		\begin{array}{l}
		\unitL,
		p \composeL c \composeL q \composeL r
		, \lmod{}, \gmod
		\end{array}
		\hspace*{-0.15cm}
		\right)
		&
		\hspace*{-0.1cm}
		\begin{array}{l}

			
			(p \composeL c), \lenv |=_{(p \composeL c \composeL q \composeL r), \lmod, \gmod} P \\
			\land (q \composeL c), \lenv |=_{(p \composeL c \composeL q \composeL r), \lmod, \gmod} Q \\
			
			\land r \in \LStates\\
			
			\land \extendsAM{\lmod{}, \gmod}{p \composeL c}{\ q \composeL r}{\semI[\lenv]{I_1}}\\
			
			\land \extendsAM{\lmod{}, \gmod}{c \composeL q}{\ p \composeL r}{\semI[\lenv]{I_2}}

		\end{array}
		\hspace*{-0.1cm}
	\end{array}
	\hspace*{-0.2cm}
	\right\} \vspace*{3pt}\\
	
	
	
	
	\text{By Lemma \ref{lem:amodMerge}} \subseteq & 
	 \left\{
	\hspace*{-0.2cm}
	\begin{array}{l | l}
		\left(
		\hspace*{-0.15cm}
		\begin{array}{l}
		\unitL,
		p \composeL c \composeL q \composeL r
		, \lmod{}, \gmod
		\end{array}
		\hspace*{-0.15cm}
		\right)
		&
		\hspace*{-0.1cm}
		\begin{array}{l}
			(p \composeL c), \lenv |=_{(p \composeL c \composeL q \composeL r), \lmod, \gmod} P \\
			\land (q \composeL c), \lenv |=_{(p \composeL c \composeL q \composeL r), \lmod, \gmod} Q \\
			
			\land r \in \LStates \\
			
			\land  \extendsAM{\lmod{}, \gmod}{p \composeL c \composeL q}{r}{\semI[\lenv]{I_1 \cup I_2}}
		\end{array}
		\hspace*{-0.1cm}
	\end{array}
	\hspace*{-0.2cm}
	\right\} \\
	
	
	
	
	
	\subseteq & 
	\left\{
	\hspace*{-0.2cm}
	\begin{array}{l | l}
		\left(
		\hspace*{-0.15cm}
		\begin{array}{l}
		\unitL,
		pq \composeL r
		, \lmod{}, \gmod
		\end{array}
		\hspace*{-0.15cm}
		\right)
		&
		\hspace*{-0.1cm}
		\begin{array}{l}
%			\left(
%			\hspace*{-0.15cm}
%			\begin{array}{l}
%				pq, 
%				(pq \composeL r)
%				, \lmod{}, \gmod
%			\end{array}
%			\hspace*{-0.15cm}
%			\right), \lenv |= P \sepish Q \\
			
			pq, \lenv |=_{pq \composeL r), \lmod, \gmod} P \sepish Q \\
			
			\land r \in \LStates \\
			\land \extendsAM{\lmod{}, \gmod}{pq}{r}{\semI[\lenv]{I_1 \cup I_2}}
		\end{array}
		\hspace*{-0.1cm}
	\end{array}
	\hspace*{-0.2cm}
	\right\} \vspace*{3pt}\\
	
	

	
	= & \left\{ w \mid w, \lenv |= \shared{P \sepish Q}{I_1 \cup I_2}\right\}
\end{array}
\]
%
\end{proof}
%
\end{lemma}
%
%
\begin{lemma}[Shift]
%
\[
	\shared{P}{I} \land I \weakenI{P} I' \semimplies \shared{P}{I'}
\]
%
\noindent\textbf{RTS.} for all $\lenv \in \LEnv$ and $w_1 \in \Worlds$, 
\[
\begin{array}{l l}
	\text{if} & w_1, \lenv |= \shared{P}{I} \land \semI[\lenv]{I} \weakenI{\left\{s \mid s, \lenv \slsat P \right\} } \semI[\lenv]{I'}\\
	\text{then} & \exsts{w_2} \heapPart{(\collapseW{w_1})} = \heapPart{(\collapseW{w_2})} \land (w_1, w_2) \in \guarantee
\end{array}
\]
%
\begin{proof}
Pick an arbitrary $w_1 = (l, g, \lmod, \gmod)$ such that 
%
\begin{align}
	& w_1, \lenv |= \shared{P}{I}  \label{shift:ass1}\\
	& \semI[\lenv]{I} \weakenI{\left\{s \mid s, \lenv \slsat P \right\} } \semI[\lenv]{I'} \label{shift:ass2}
\end{align}
%
and let $w_2 = (l, g, \lmod \cup \semI[\lenv]{I'}, \gmod)$. Then by definition of $\collapseW{.}$ we have 
%
\begin{equation}
	\heapPart{(\collapseW{w_1})} = \heapPart{(\collapseW{w_2})} \label{shift:goal1}
\end{equation}
%
On the other hand from Lemma \ref{lem:amodHiding} and \ref{shift:ass2} we have: 
%	
\begin{equation}
	\for{s, r, \lmod'} s \composeL = g \land \extendsAM{\lmod, \gmod}{s}{r}{\lmod'} \implies \extendsAM{\lmod \cup \lmod_{0}, \gmod}{s}{r}{\lmod'}  \label{shift:ass3}
\end{equation}
%
From \ref{shift:ass3} and the definitions of $w_1$ and $w_2$ we have: 
%
\begin{equation}
	(w_1, w_2) \in \shiftG \nonumber
\end{equation}
%
and consequently
%
\begin{equation}
	(w_1, w_2) \in \guarantee \nonumber
\end{equation}
%
as required.

\end{proof}
\end{lemma}
%
%
%
\begin{lemma}[] \label{lem:extension}
%
\[
		P \containI I  \Rrightarrow \exsts{\capAss{1}, \capAss{2}} \;\; \capAss{1} * \shared{P * \capAss{2}}{I}
\]
%
\begin{proof}
\textbf{RTS. }
%
\[
\begin{array}{l}
	\for{\lenv} \for{w_1} w_1, \lenv |=  P \implies\\
	\hspace{0.2cm} \exsts{w_2} w_2, \lenv |= \exsts{\capAss{1}} \;\; \capAss{1} * \shared{P * \capAss{2}}{I} \land \\
	\hspace*{0.4cm} (w_1, w_2) \in \guarantee \;\land\; \heapPart{\left(\collapseW{w_1}\right)} = \heapPart{\left(\collapseW{w_2}\right)}
\end{array}
\]
%
Pick an arbitrary $\lenv$, $w_1 = (l, g, \lmod{}, \gmod)$ such that $w, \lenv |= P$ and set $K$ such that:
\begin{align}
%	K = 
%	\semK[\lenv]{\left( \bigvee\limits_{\lambda \vec{x}. \capAss{}: a \in \dom{I}} \capAss{}\right) \;\lor\; \capAss{1} }
%	\;\land\; K \disjoint \dom{\amod{L}} \label{LE:Ass1}
	K = 
	\semK[\lenv]{\capAss{1} \lor \capAss{2}}
	\;\land\; K \disjoint \dom{\amod{L}} \label{LE:Ass1}
\end{align}	 
%
Since $\wf{w_1}$, we know 
\begin{align}
	\exsts{\fence{L}} g \in \fence{L} \;\land\; \fence{L} \strictfences \amod{L} \label{LE:Ass2}
\end{align} 
%Pick arbitrary $l_1, \cdots, l_n \in \LStates$, $\amod{1} , \cdots, \amod{n} \in \AMods$, $F_1, \cdots, F_n \in \pset{\LStates}$ such that 
%%
%\begin{align}
%\begin{array}{l}
%	l_1 \composeL \cdots \composeL l_n = s \\
%	\for{\amod{i}, \amod{j} \in \left(\amod{1} \cup \cdots \cup \amod{n}\right)} \dom{\amod{i}} \disjoint \dom{\amod{j}}\\
%	\dom{\amod{}} = \dom{\amod{1}} \cup \cdots \cup \dom{\amod{n}}\\
%	\for{i \in 1, \cdots, n} l_i \in F_i \;\land\; F_i \strictfences \amod{i}\;\land\;\\
%	\hspace*{1cm}\extendsAM{\amod{}}{l_i}{l_1 \composeL \cdots \composeL l_{i-1} \composeL l_{i+1} \composeL \cdots \composeL l_n}{\amod{i}} \label{LE:Ass2}
%\end{array}
%\end{align}
%%
On the other hand, from the premise of the lemma we know 
%
\begin{align}
	\exsts{\fence{}} l \in \fence{} \;\land\; \fence{} \strictfences \semI[\lenv]{I} \label{LE:Ass3}
\end{align}
%(\ref{LE:Ass})
Since $\wf{w_1}$, we know $l \composeL g \text{ is defined}$ and thus from (\ref{LE:Ass1})-(\ref{LE:Ass3}) and lemma \ref{lem:amodWitness} we know:
%
\begin{align}
\begin{array}{l}
	\exsts{\gmod', \fence{}'} l \composeL g \in \fence{}' \;\land\; \fence{}' \strictfences \lmod \cup \semI[\lenv]{I} \;\land\; \extendsAM{\lmod \cup \semI[\lenv]{I}, \gmod'}{l}{g}{\semI[\lenv]{I}} \;\land\\
	\hspace*{1.3cm}\for{s', r'} \for{\lmod_{1} \subseteq \lmod} s' \composeL r' = g \;\land\; \extendsAM{\lmod{}, \gmod}{s'}{r'}{\lmod_{1}} \implies\\
	\hspace*{1.8cm}\extendsAM{\lmod \cup \semI[\lenv]{I}, \gmod'}{s'}{r' \composeL l}{\lmod_{1}} 
\end{array}\label{LE:Ass4}
\end{align}
%
%Pick $\amod{}'$ such that (\ref{LE:Ass4}) is satisfied. Then from (\ref{LE:Ass2}) and (\ref{LE:Ass4}) we know
%%
%\begin{align}
%	\expandsAM{\amod{}'}{s}{l}{\amod{}} \;\land\; \extendsAM{\amod{}'}{l}{s}{\intermediateSemI{I}} \label{LE:Ass5}
%\end{align}
%%
Pick $\gmod'$ such that (\ref{LE:Ass4}) is satisfied. Pick $\ca{1} \in \semK[\lenv]{\capAss{1}}$, $\ca{2} \in \semK[\lenv]{\capAss{2}}$ and $w_2 = ( (\unitH, \ca{1}), l \composeL g \composeL (\unitH, \ca{2}), \lmod\cup \intermediateSemI{I}, \gmod' )$. Then from (\ref{LE:Ass1}) and (\ref{LE:Ass4}) we know
%
\begin{align}
	(w_1, w_2) \in \guarantee \label{LE:Ass6}
\end{align}
%
On the other hand, from the definition of $\collapseW{.}$ we know:
%(\ref{LE:Ass})
\begin{align}
	\heapPart{\left(\collapseW{w_1}\right)} = \heapPart{\left(\collapseW{w_2}\right)} \label{LE:Ass7}
\end{align}
%
Finally since $w_2, \lenv |= \capAss{1} * \shared{P * \capAss{2}}{I}$, from (\ref{LE:Ass6}) and (\ref{LE:Ass7}) we have
%
\begin{align}
	(w_1, w_2) \in \guarantee \;\land\; \heapPart{\left(\collapseW{w_1}\right)} = \heapPart{\left(\collapseW{w_2}\right)}
\end{align}
%
as required.
\end{proof}
\end{lemma}
%

\input{Soundness/auxiliaryLemmas.tex}

