\begin{lemma}\label{lem:existential-promotion}
Given any assertion $P \in \Assertions$, the following is valid.
%
\[
	P <=> \promote{P}
\]
%
\begin{proof}
\todo
\end{proof}
\end{lemma}
%
%
\begin{lemma}[]\label{lem:sub-stable-extend}
for all $P \in \Assertions$, $\lenv \in \LEnv$, $w, w' \in \Worlds$, 
% 
\[
\begin{array}{@{} l @{}}
	w, \lenv |= P /| (w, w') \in \extendR 
	\implies  w', \lenv |= P
\end{array}
\]
%
\begin{proof}
From the definition of $\extendR$, it then suffices to show that for all $P \in \Assertions$, $\lenv \in \LEnv$, $l, g, g' \in \LStates$ and $\lmod, \lmod' \in \AMods$: 
% 
\[
\begin{array}{@{} l @{}}
	(l, g, \lmod), \lenv |= P /| 
	\expandsAM{\lmod'}{g'}{g}{\lmod}
	 \implies  (l, g \composeL g', \lmod \cup \lmod'), \lenv |= P
\end{array}
\]
%
We proceed by induction on the structure of assertion $P$.	\\

\noindent\textbf{Case $P \eqdef A$\quad} Immediate.\\
\noindent\textbf{Case $P \eqdef P_1 \implies P_2$} \\
Pick an arbitrary $\lenv \in \LEnv$, $l, g, g' \in \LStates$ and $\lmod, \lmod' \in \AMods$ such that
%
\begin{align}
	& (l, g, \lmod), \lenv |= P_1 \lor P_2 \label{sub-stable-extend:Ass1}\\
%	
	&\expandsAM{\lmod'}{g'}{g}{\lmod} \label{sub-stable-extend:Ass2}\\
%	
	& \for{l, g, g' \in \LStates} \for{\lmod', \lmod\in \AMods} \nonumber\\
	\tag{I.H1} & 
	\quad (l, g, \lmod), \lenv |= P_1 /| \expandsAM{\lmod'}{g'}{g}{\lmod} \implies (l, g \composeL g', \lmod \cup \lmod'), \lenv |= P_1 \label{sub-stable-extend:IH1}\\ 
%
	& \for{l, g, g' \in \LStates} \for{\lmod', \lmod \in \AMods} \nonumber\\
	\tag{I.H2} & 
	\quad (l, g, \lmod), \lenv |= P_2 /| \expandsAM{\lmod'}{g'}{g}{\lmod} \implies (l, g \composeL g', \lmod \cup \lmod'), \lenv |= P_2 \label{sub-stable-extend:IH2}
%	
\end{align}
%
From (\ref{sub-stable-extend:Ass1}) and the definition of $|=$ we know $(l, g, \lmod), \lenv |= P_1$ \text{ or } $(l, g, \lmod), \lenv |= P_2$; consequently, from (\ref{sub-stable-extend:Ass2}), (\ref{sub-stable-extend:IH1}) and (\ref{sub-stable-extend:IH2}) we have: $(l, g \composeL g', \lmod \cup \lmod'), \lenv |= P_1$ \text{ or } $(l, g \composeL g', \lmod \cup \lmod'), \lenv |= P_2$. Thus, from the definition of $|=$ we have:
%
\begin{align*}
	(l, g \composeL g', \lmod \cup \lmod'), \lenv |= P_1 \lor P_2
\end{align*}
%
as required.\\

\noindent\textbf{Cases $P \eqdef \exsts{x} P'$; $P \eqdef P_1 * P_2$; $P \eqdef P_1 ** P_2$; $P \eqdef P_1 \land P_2$} \\
These cases are analogous to the previous case and are omitted here. \\

\noindent\textbf{Case $P \eqdef \shared{P'}{I}$} \\
Pick an arbitrary $\lenv \in \LEnv$, $s, g \in \LStates$ and $\lmod, \lmod' \in \AMods$ such that
%
\begin{align}
	&(l, g, \lmod), \lenv |= \shared{P'}{I} \label{sub-stable-extend:Ass3}\\
	& \expandsAM{\lmod'}{g'}{g}{\lmod} \label{sub-stable-extend:Ass4}\\
	& \for{l, g , g'\in \LStates} \for{\lmod', \lmod \in \AMods} \nonumber\\
	\tag{I.H} & 
	\quad (l, g, \lmod), \lenv |= P' /| \expandsAM{\lmod'}{g'}{g}{\lmod} \implies (l, g \composeL g', \lmod \cup \lmod'), \lenv |= P' \label{sub-stable-extend:IH}
\end{align}
%
From (\ref{sub-stable-extend:Ass3}) and the definition of $|=$ we have:
%
\begin{align*}
	l = \unitL /| \exsts{s', r'} g = s' \composeL r' /| s', \lenv |=_{g, \lmod} P' /| \extendsAM{\lmod}{s'}{r'}{\semI[\lenv]{I}} 
\end{align*}  
%
Thus from (\ref{sub-stable-extend:Ass4}) and \lem~\ref{lem:sub-stable-1} we have
%
\begin{align*}
	& l = \unitL /| \exsts{s', r'} g \composeL g' = s' \composeL r' \composeL g' /| s', \lenv |=_{g \composeL g', \lmod \cup \lmod'} P' /|\\
	& \extendsAM{\lmod}{s'}{r'}{\semI[\lenv]{I}}
\end{align*}
%
and consequently from (\ref{sub-stable-extend:Ass4}) and (\ref{sub-stable-extend:IH}) we have
%
\begin{align*}
	& l = \unitL /| \exsts{s', r'} g \composeL g' = s' \composeL r' /| s', \lenv |=_{g \composeL g', \lmod \cup \lmod'} P' /|\\
	& \extendsAM{\lmod \cup \lmod'}{s'}{r'}{\semI[\lenv]{I}}
\end{align*}
%
That is,
%%
%\begin{align*}
%	(s, g, \lmod \cup \lmod', \gmod'), \lenv |= \shared{P'}{I}
%\end{align*}
%%
%and consequently, from the semantics of $|=_{g, \lmod \cup \lmod', \gmod'}$
%
\begin{align}
	(l, g \composeL g', \lmod \cup \lmod'), \lenv |= \shared{P'}{I} \label{sub-stable-extend:Ass5}
\end{align}
%
as required.
\end{proof}
\end{lemma}
%
%
\begin{lemma}[]\label{lem:sub-stable-1}
for all $P \in \Assertions$, $\lenv \in \LEnv$, $s, g, g' \in \LStates$ and $\lmod, \lmod' \in \AMods$: 
% 
\[
\begin{array}{@{} l @{}}
	s, \lenv |=_{g, \lmod} P /| 
	\expandsAM{\lmod'}{g'}{g}{\lmod}
	 \implies  s, \lenv |=_{g \composeL g', \lmod \cup \lmod'} P
\end{array}
\]
%
\begin{proof}
By induction on the structure of assertion $P$.	\\

\noindent\textbf{Case $P \eqdef A$\quad} Immediate.\\
\noindent\textbf{Case $P \eqdef P_1 \implies P_2$} \\
Pick an arbitrary $\lenv \in \LEnv$, $s, g, g' \in \LStates$ and $\lmod, \lmod' \in \AMods$ such that
%
\begin{align}
	& s, \lenv |=_{g, \lmod} P_1 \implies P_2 \label{subextend2:Ass1}\\
%	
	&\expandsAM{\lmod'}{g'}{g}{\lmod} \label{subextend2:Ass2}\\
%	
	& \for{s, g, g' \in \LStates} \for{\lmod', \lmod \in \AMods} \nonumber\\
	\tag{I.H1} & 
	\quad s, \lenv |=_{g, \lmod} P_1 /| \expandsAM{\lmod'}{g'}{g}{\lmod} \implies s, \lenv |=_{g \composeL g', \lmod \cup \lmod'} P_1 \label{subextend2:IH1}\\ 
%
	& \for{s, g, g' \in \LStates} \for{\lmod', \lmod \in \AMods} \nonumber\\
	\tag{I.H2} & 
	\quad s, \lenv |=_{g, \lmod} P_2 /| \expandsAM{\lmod'}{g'}{g}{\lmod} \implies s, \lenv |=_{g \composeL g', \lmod \cup \lmod'} P_2 \label{subextend2:IH2}
%	
\end{align}
%
From (\ref{subextend2:Ass1}) and the definition of $|=_{g, \lmod}$ we know $s, \lenv |=_{g, \lmod} P_1$ \text{ implies } $P_2 |=_{g, \lmod}$; consequently, from (\ref{subextend2:Ass2}), (\ref{subextend2:IH1}) and (\ref{subextend2:IH2}) we have: $s, \lenv |=_{g \composeL g', \lmod \cup \lmod'} P_1$ \text{ implies } $s, \lenv |=_{g \composeL g', \lmod \cup \lmod'} P_2$. Thus, from the definition of $|=_{g \composeL g', \lmod \cup \lmod'}$ we have:
%
\begin{align*}
	s, \lenv |=_{g \composeL g', \lmod \cup \lmod'} P_1 \implies P_2
\end{align*}
%
as required.\\

\noindent\textbf{Cases $P \eqdef \exsts{x} P'$; $P \eqdef P_1 * P_2$; $P \eqdef P_1 ** P_2$} \\
These cases are analogous to the previous case and are omitted here. \\

\noindent\textbf{Case $P \eqdef \shared{P'}{I}$} \\
Pick an arbitrary $\lenv \in \LEnv$, $s, g \in \LStates$ and $\lmod, \lmod' \in \AMods$ such that
%
\begin{align}
	&s, \lenv |=_{g, \lmod} \shared{P'}{I} \label{subextend2:Ass3}\\
	& \expandsAM{\lmod'}{g'}{g}{\lmod} \label{subextend2:Ass4}\\
	& \for{s, g , g'\in \LStates} \for{\lmod', \lmod \in \AMods} \nonumber\\
	\tag{I.H} & 
	\quad s, \lenv |=_{g, \lmod} P' /| \expandsAM{\lmod'}{g'}{g}{\lmod} \implies s, \lenv |=_{g \composeL g', \lmod \cup \lmod'} P' \label{subextend2:IH}
\end{align}
%
From (\ref{subextend2:Ass3}) and the definition of $|=_{g, \lmod}$ we have:
%
\begin{align*}
	s = \unitL /| \exsts{s', r'} g = s' \composeL r' /| s', \lenv |=_{g, \lmod} P' /| \extendsAM{\lmod}{s'}{r'}{\semI[\lenv]{I}} 
\end{align*}  
%
Thus from (\ref{subextend2:Ass4}) and (\ref{subextend2:IH}) we have
%
\begin{align*}
	& s = \unitL /| \exsts{s', r'} g \composeL g' = s' \composeL r' /| s', \lenv |=_{g \composeL g', \lmod \cup \lmod'} P' /|\\
	& \extendsAM{\lmod \cup \lmod'}{s'}{r'}{\semI[\lenv]{I}}
\end{align*}
%
That is,
%%
%\begin{align*}
%	(s, g, \lmod \cup \lmod', \gmod'), \lenv |= \shared{P'}{I}
%\end{align*}
%%
%and consequently, from the semantics of $|=_{g, \lmod \cup \lmod', \gmod'}$
%
\begin{align*}
	s, \lenv |=_{g, \lmod \cup \lmod'} \shared{P'}{I}
\end{align*}
%
as required.
\end{proof}
%
\end{lemma}
%
%
\begin{lemma}[]\label{lem:sub-stable-shift}
for all $P \in \Assertions$, $\lenv \in \LEnv$, $w, w' \in \Worlds$, 
% 
\[
\begin{array}{@{} l @{}}
	w, \lenv |= P /| (w, w') \in \shiftR 
	\implies  w', \lenv |= P
\end{array}
\]
%
\begin{proof}
From the definition of $\shiftR$, it then suffices to show that for all $P \in \Assertions$, $\lenv \in \LEnv$, $l, g, \in \LStates$ and $\lmod, \lmod' \in \AMods$: 
% 
\[
\begin{array}{@{} l @{}}
	(l, g, \lmod), \lenv |= P /| 
	\expandsAM{\lmod'}{\unitL}{g}{\lmod}
	 \implies  (l, g, \lmod \cup \lmod'), \lenv |= P
\end{array}
\]
%
This follows immediately from the more general result established in \lem~\ref{lem:sub-stable-extend} from (\ref{sub-stable-extend:Ass1}) to (\ref{sub-stable-extend:Ass5}).
\end{proof}
%
\end{lemma}
%
%
\begin{lemma}[]\label{lem:extend1}
for all $P \in \Assertions$, $\lenv \in \LEnv$, $s, g \in \LStates$ and $\lmod, \lmod' \in \AMods$: 
% 
\[
\begin{array}{@{} l @{}}
	(s, g, \lmod), \lenv |= P /| \expandsAM{\lmod'}{s}{g}{\lmod}
	\implies  s, \lenv |=_{g \composeL s, \lmod \cup \lmod'} P
\end{array}
\]
%
\begin{proof}
By induction on the structure of assertion $P$.	\\

\noindent\textbf{Case $P \eqdef A$\quad} Immediate.\\
\noindent\textbf{Case $P \eqdef P_1 \implies P_2$} \\
Pick an arbitrary $\lenv \in \LEnv$, $s, g \in \LStates$ and $\lmod, \lmod' \in \AMods$ such that
%
\begin{align}
	& (s, g, \lmod), \lenv |= P_1 \implies P_2 \label{subextend:Ass1}\\
%	
	& \expandsAM{\lmod'}{s}{g}{\lmod} \label{subextend:Ass2}\\
%	
	& \for{s, g \in \LStates} \for{\lmod, \lmod' \in \AMods} \nonumber\\
	\tag{I.H1} & \quad (s, g, \lmod), \lenv |= P_1 /| \expandsAM{\lmod'}{s}{g}{\lmod}
	\implies s, \lenv |=_{g \composeL s, \lmod \cup \lmod'} P_1
	\label{subextend:IH1}\\ 
%
	& \for{s, g \in \LStates} \for{\lmod, \lmod' \in \AMods} \nonumber\\
	\tag{I.H2} & \quad (s, g, \lmod), \lenv |= P_2 /| \expandsAM{\lmod'}{s}{g}{\lmod}
	\implies s, \lenv |=_{g \composeL s, \lmod \cup \lmod'} P_2
	\label{subextend:IH2}
%	
\end{align}
%
From (\ref{subextend:Ass1}) and the definition of $|=$ we know $(s, g, \lmod), \lenv |= P_1$ \text{ implies } $(s, g, \lmod), \lenv |= P_2$; consequently, from (\ref{subextend:Ass2}), (\ref{subextend:IH1}) and (\ref{subextend:IH2}) we have: $s, \lenv |=_{g \composeL s, \lmod \cup \lmod'} P_1$ \text{ implies } $s, \lenv |=_{g \composeL s, \lmod \cup \lmod'} P_2$. Thus, from the definition of $|=_{g \composeL s, \lmod \cup \lmod'}$ we have:
%
\begin{align*}
	s, \lenv |=_{g \composeL s, \lmod \cup \lmod'} P_1 \implies P_2
\end{align*}
%
as required.\\

\noindent\textbf{Cases $P \eqdef \exsts{x} P'$; $P \eqdef P_1 * P_2$; $P \eqdef P_1 ** P_2$} \\
These cases are analogous to the previous case and are omitted here. \\

\noindent\textbf{Case $P \eqdef \shared{P'}{I}$} \\
Pick an arbitrary $\lenv \in \LEnv$, $s, g \in \LStates$ and $\lmod, \lmod' \in \AMods$ such that
%
\begin{align}
	& (s, g, \lmod), \lenv |= \shared{P'}{I} \label{subextend:Ass3}\\
	& \expandsAM{\lmod'}{s}{g}{\lmod} \label{subextend:Ass4}
%	\\
%	& \for{s, g \in \LStates} \for{\lmod, \lmod', \gmod, \gmod' \in \AMods} \nonumber\\
%	\tag{I.H} & \quad s, \lenv |=_{g, \lmod, \gmod} P' /| \expandsAM{\gmod'}{s}{\lmod'}{g}{\lmod}{\gmod} 
%	\implies s, \lenv |=_{g \composeL s, \lmod \cup \lmod', \gmod'} P'
%	\label{subextend:IH}
\end{align}
%
From (\ref{subextend:Ass3}) and the definition of $|=$ we have:
%
\begin{align*}
	s = \unitL /| \exsts{s', r'} g = s' \composeL r' /| s', \lenv |=_{g, \lmod} P' /| \extendsAM{\lmod}{s'}{r'}{\semI[\lenv]{I}} 
\end{align*}  
%
Thus from (\ref{subextend:Ass4}) we have
%
\begin{align*}
	s = \unitL /| \exsts{s', r'} g = s' \composeL r' /| s', \lenv |=_{g, \lmod} P' /| \extendsAM{\lmod \cup \lmod'}{s'}{r' \composeL s}{\semI[\lenv]{I}}
\end{align*}
%
and consequently from (\ref{subextend:Ass4}), \lem~\ref{lem:sub-stable-1} and since $s = \unitL$
%
\begin{align*}
	& s = \unitL /| \exsts{s', r'} g \composeL s = s' \composeL r' /| s', \lenv |=_{g \composeL s, \lmod \cup \lmod'} P'  \\
	& /| \extendsAM{\lmod \cup \lmod'}{s'}{r' \composeL s}{\semI[\lenv]{I}}
\end{align*}
That is,
%
%\begin{align*}
%	(s, g, \lmod \cup \lmod', \gmod), \lenv |= \shared{P'}{I}
%\end{align*}
%%
%and consequently, from the semantics of $|=_{g, \lmod \cup \lmod', \gmod}$
%
\begin{align*}
	s, \lenv |=_{g \composeL s, \lmod \cup \lmod'} \shared{P'}{I}
\end{align*}
%
as required.
\end{proof}
\end{lemma}
%
